Progress on Kraus maps.

isabelle-thys/Programs.thy
@@ -3,54 +3,6 @@ theory Programs
 begin
 
 (* TODO move *)
-instantiation trace_class :: (chilbert_space, chilbert_space) order begin
-lift_definition less_eq_trace_class :: \<open>('a, 'b) trace_class \<Rightarrow> ('a, 'b) trace_class \<Rightarrow> bool\<close> is
-  less_eq.
-lift_definition less_trace_class :: \<open>('a, 'b) trace_class \<Rightarrow> ('a, 'b) trace_class \<Rightarrow> bool\<close> is
-  less.
-instance
-  apply intro_classes
-     apply (auto simp add: less_eq_trace_class.rep_eq less_trace_class.rep_eq)
-  by (simp add: from_trace_class_inject)
-end
-
-type_synonym ('a,'b) kraus_family = \<open>('a \<Rightarrow>\<^sub>C\<^sub>L 'b) \<Rightarrow> nat\<close>
-
-definition \<open>kraus_family \<EE> \<longleftrightarrow> (\<exists>B. \<forall>F. finite F \<longrightarrow> norm (\<Sum>E\<in>F. \<EE> E *\<^sub>C (E* o\<^sub>C\<^sub>L E)) \<le> B)\<close>
-  for \<EE> :: \<open>(_::chilbert_space, _::chilbert_space) kraus_family\<close>
-definition \<open>krause_norm \<EE> = (SUP F\<in>Collect finite. norm (\<Sum>E\<in>F. \<EE> E *\<^sub>C (E* o\<^sub>C\<^sub>L E)))\<close>
-
-definition \<open>kraus_family_map \<EE> \<rho> = (\<Sum>\<^sub>\<infinity>E. of_nat (\<EE> E) *\<^sub>C Abs_trace_class (E o\<^sub>C\<^sub>L from_trace_class \<rho> o\<^sub>C\<^sub>L E*))\<close>
-
-definition \<open>kraus_equivalent \<EE> \<FF> \<longleftrightarrow> kraus_family \<EE> \<and> kraus_family \<FF> \<and> kraus_family_map \<EE> = kraus_family_map \<FF>\<close>
-
-lemma kraus_family_zero[simp]: \<open>kraus_family (\<lambda>_. 0)\<close>
-  by (auto simp: kraus_family_def)
-
-quotient_type (overloaded) ('a,'b) kraus_map = \<open>('a::chilbert_space, 'b::chilbert_space) kraus_family\<close> / partial: kraus_equivalent
-  by (auto intro!: part_equivpI exI[of _ \<open>\<lambda>_. 0\<close>] sympI transpI simp: kraus_equivalent_def)
-
-definition \<open>kraus_family_comp \<EE> \<FF> G = (if G=0 then 0 else \<Sum>(E,F)|(\<EE> E \<noteq> 0 \<and> \<FF> F \<noteq> 0 \<and> E o\<^sub>C\<^sub>L F = G). \<EE> E * \<FF> F)\<close> 
-\<comment> \<open>The lemma \<open>kraus_family_comp_finite\<close> below shows that we range over a finite set in the sum.\<close>
-  for \<EE> \<FF> :: \<open>(_::chilbert_space, _::chilbert_space) kraus_family\<close>
-
-definition kraus_family_of_op :: \<open>_ \<Rightarrow> (_::chilbert_space,_::chilbert_space) kraus_family\<close> where
-  \<open>kraus_family_of_op E F = (if E=F then 1 else 0)\<close>
-
-lemma kraus_family_kraus_family_of_op[simp]: \<open>kraus_family (kraus_family_of_op E)\<close>
-proof -
-  have \<open>(\<Sum>F\<in>M. kraus_family_of_op E F *\<^sub>C (F* o\<^sub>C\<^sub>L F)) = (if E\<in>M then E* o\<^sub>C\<^sub>L E else 0)\<close> if \<open>finite M\<close> for M
-    apply (subst sum_single[where i=E])
-    using that by (auto simp: kraus_family_of_op_def)
-  then show ?thesis
-    by (auto simp add: kraus_family_def)
-qed
-
-lift_definition kraus_map_of_op :: \<open>('a::chilbert_space \<Rightarrow>\<^sub>C\<^sub>L 'b::chilbert_space) \<Rightarrow> ('a,'b) kraus_map\<close>
-  is kraus_family_of_op
-  by (simp add: kraus_equivalent_def)
-
-(* TODO move *)
 lemma norm_cblinfun_mono:
   fixes A B :: \<open>'a::chilbert_space \<Rightarrow>\<^sub>C\<^sub>L 'a\<close>
   assumes \<open>A \<ge> 0\<close>
@@ -78,14 +30,685 @@ proof -
     by force
 qed
 
+lemma sandwich_mono: \<open>sandwich A B \<le> sandwich A C\<close> if \<open>B \<le> C\<close>
+  by (metis cblinfun.real.diff_right diff_ge_0_iff_ge sandwich_pos that)
+
+lemma abs_op_id_on_pos: \<open>a \<ge> 0 \<Longrightarrow> abs_op a = a\<close>
+  using abs_opI by force
+
+lemma cmod_mono: \<open>0 \<le> a \<Longrightarrow> a \<le> b \<Longrightarrow> cmod a \<le> cmod b\<close>
+  by (simp add: cmod_Re less_eq_complex_def)
+
+lemma trace_norm_bounded:
+  fixes A B :: \<open>'a::chilbert_space \<Rightarrow>\<^sub>C\<^sub>L 'a\<close>
+  assumes \<open>A \<ge> 0\<close> and \<open>trace_class B\<close>
+  assumes \<open>A \<le> B\<close>
+  shows \<open>trace_class A\<close>
+proof -
+  have \<open>(\<lambda>x. x \<bullet>\<^sub>C (B *\<^sub>V x)) abs_summable_on some_chilbert_basis\<close>
+    by (metis assms(2) is_onb_some_chilbert_basis summable_on_iff_abs_summable_on_complex trace_exists)
+  then have \<open>(\<lambda>x. x \<bullet>\<^sub>C (A *\<^sub>V x)) abs_summable_on some_chilbert_basis\<close>
+    apply (rule abs_summable_on_comparison_test)
+    using \<open>A \<ge> 0\<close> \<open>A \<le> B\<close>
+    by (auto intro!: cmod_mono cinner_pos_if_pos simp: abs_op_id_on_pos less_eq_cblinfun_def)
+  then show ?thesis
+    by (auto intro!: trace_classI[OF is_onb_some_chilbert_basis] simp: abs_op_id_on_pos \<open>A \<ge> 0\<close>)
+qed
+
+lemma trace_norm_cblinfun_mono:
+  fixes A B :: \<open>'a::chilbert_space \<Rightarrow>\<^sub>C\<^sub>L 'a\<close>
+  assumes \<open>A \<ge> 0\<close> and \<open>trace_class B\<close>
+  assumes \<open>A \<le> B\<close>
+  shows \<open>trace_norm A \<le> trace_norm B\<close>
+proof -
+  from assms have \<open>trace_class A\<close>
+    by (rule trace_norm_bounded)
+  from \<open>A \<le> B\<close> and \<open>A \<ge> 0\<close>
+  have \<open>B \<ge> 0\<close>
+    by simp
+  have \<open>cmod (x \<bullet>\<^sub>C (abs_op A *\<^sub>V x)) \<le> cmod (x \<bullet>\<^sub>C (abs_op B *\<^sub>V x))\<close> for x
+    using \<open>A \<le> B\<close>
+    unfolding less_eq_cblinfun_def
+    using \<open>A \<ge> 0\<close> \<open>B \<ge> 0\<close> 
+    by (auto intro!: cmod_mono cinner_pos_if_pos simp: abs_op_id_on_pos)
+  then show \<open>trace_norm A \<le> trace_norm B\<close>
+    using \<open>trace_class A\<close> \<open>trace_class B\<close>
+    by (auto intro!: infsum_mono 
+        simp add: trace_norm_def trace_class_iff_summable[OF is_onb_some_chilbert_basis])
+qed
+
+(* TODO move *)
+instantiation trace_class :: (chilbert_space, chilbert_space) order begin
+lift_definition less_eq_trace_class :: \<open>('a, 'b) trace_class \<Rightarrow> ('a, 'b) trace_class \<Rightarrow> bool\<close> is
+  less_eq.
+lift_definition less_trace_class :: \<open>('a, 'b) trace_class \<Rightarrow> ('a, 'b) trace_class \<Rightarrow> bool\<close> is
+  less.
+instance
+  apply intro_classes
+     apply (auto simp add: less_eq_trace_class.rep_eq less_trace_class.rep_eq)
+  by (simp add: from_trace_class_inject)
+end
+
+
+lemma norm_cblinfun_mono_trace_class:
+  fixes A B :: \<open>('a::chilbert_space, 'a) trace_class\<close>
+  assumes \<open>A \<ge> 0\<close>
+  assumes \<open>A \<le> B\<close>
+  shows \<open>norm A \<le> norm B\<close>
+  using assms
+  apply transfer
+  apply (rule trace_norm_cblinfun_mono)
+  by auto
+
+type_synonym ('a,'b) kraus_family = \<open>('a \<Rightarrow>\<^sub>C\<^sub>L 'b) \<Rightarrow> nat\<close>
+
+definition \<open>kraus_family \<EE> \<longleftrightarrow> (\<exists>B. \<forall>F. finite F \<longrightarrow> norm (\<Sum>E\<in>F. \<EE> E *\<^sub>C (E* o\<^sub>C\<^sub>L E)) \<le> B)\<close>
+  for \<EE> :: \<open>(_::chilbert_space, _::chilbert_space) kraus_family\<close>
+definition \<open>kraus_family_norm \<EE> = (SUP F\<in>Collect finite. norm (\<Sum>E\<in>F. complex_of_nat (\<EE> E) *\<^sub>C (E* o\<^sub>C\<^sub>L E)))\<close>
+
+definition \<open>kraus_family_map \<EE> \<rho> = (\<Sum>\<^sub>\<infinity>E. of_nat (\<EE> E) *\<^sub>C Abs_trace_class (E o\<^sub>C\<^sub>L from_trace_class \<rho> o\<^sub>C\<^sub>L E*))\<close>
+
+definition \<open>kraus_equivalent \<EE> \<FF> \<longleftrightarrow> kraus_family \<EE> \<and> kraus_family \<FF> \<and> kraus_family_map \<EE> = kraus_family_map \<FF>\<close>
+
+lemma kraus_family_zero[simp]: \<open>kraus_family (\<lambda>_. 0)\<close>
+  by (auto simp: kraus_family_def)
+
+quotient_type (overloaded) ('a,'b) kraus_map = \<open>('a::chilbert_space, 'b::chilbert_space) kraus_family\<close> / partial: kraus_equivalent
+  by (auto intro!: part_equivpI exI[of _ \<open>\<lambda>_. 0\<close>] sympI transpI simp: kraus_equivalent_def)
+
+definition \<open>kraus_family_comp \<EE> \<FF> G = (if G=0 then 0 else \<Sum>(E,F)|(\<EE> E \<noteq> 0 \<and> \<FF> F \<noteq> 0 \<and> E o\<^sub>C\<^sub>L F = G). \<EE> E * \<FF> F)\<close> 
+\<comment> \<open>The lemma \<open>kraus_family_comp_finite\<close> below shows that we range over a finite set in the sum.\<close>
+  for \<EE> \<FF> :: \<open>(_::chilbert_space, _::chilbert_space) kraus_family\<close>
+
+definition kraus_family_of_op :: \<open>_ \<Rightarrow> (_::chilbert_space,_::chilbert_space) kraus_family\<close> where
+  \<open>kraus_family_of_op E F = of_bool (E=F)\<close>
+
+lemma kraus_family_kraus_family_of_op[simp]: \<open>kraus_family (kraus_family_of_op E)\<close>
+proof -
+  have \<open>(\<Sum>F\<in>M. kraus_family_of_op E F *\<^sub>C (F* o\<^sub>C\<^sub>L F)) = (if E\<in>M then E* o\<^sub>C\<^sub>L E else 0)\<close> if \<open>finite M\<close> for M
+    apply (subst sum_single[where i=E])
+    using that by (auto simp: kraus_family_of_op_def)
+  then show ?thesis
+    by (auto simp add: kraus_family_def)
+qed
+
+lemma kraus_family_of_op_norm[simp]:
+  \<open>kraus_family_norm (kraus_family_of_op E) = (norm E)\<^sup>2\<close>
+proof -
+  have \<open>kraus_family_norm (kraus_family_of_op E) = 
+      (\<Squnion>M\<in>Collect finite. norm (\<Sum>F\<in>M. of_bool (E=F) *\<^sub>C (F* o\<^sub>C\<^sub>L F)))\<close>
+    by (simp add: kraus_family_norm_def kraus_family_of_op_def)
+  also have \<open>\<dots> = (\<Squnion>M\<in>Collect finite. if E\<in>M then norm (E* o\<^sub>C\<^sub>L E) else 0)\<close>
+  proof (rule SUP_cong, simp)
+    fix M :: \<open>('a \<Rightarrow>\<^sub>C\<^sub>L 'b) set\<close> assume \<open>M \<in> Collect finite\<close>
+    then have [simp]: \<open>finite M\<close> by simp
+    show \<open>norm (\<Sum>F\<in>M. of_bool (E = F) *\<^sub>C (F* o\<^sub>C\<^sub>L F)) = (if E \<in> M then norm (E* o\<^sub>C\<^sub>L E) else 0)\<close>
+      apply (subst sum_single[where i=E])
+      by auto
+  qed
+  also have \<open>\<dots> = norm (E* o\<^sub>C\<^sub>L E)\<close>
+    apply (rule cSup_eq_maximum)
+    by auto
+  also have \<open>\<dots> = (norm E)\<^sup>2\<close>
+    by simp
+  finally show ?thesis
+    by -
+qed
+
+lift_definition kraus_map_of_op :: \<open>('a::chilbert_space \<Rightarrow>\<^sub>C\<^sub>L 'b::chilbert_space) \<Rightarrow> ('a,'b) kraus_map\<close>
+  is kraus_family_of_op
+  by (simp add: kraus_equivalent_def)
+
+lemma kraus_family_map_bounded:
+  assumes \<open>kraus_family \<EE>\<close>
+  shows \<open>norm (kraus_family_map \<EE> \<rho>) \<le> kraus_family_norm \<EE> * norm \<rho>\<close>
+  sorry
+
+lemma kraus_family_norm_geq0:
+  assumes \<open>kraus_family \<EE>\<close>
+  shows \<open>kraus_family_norm \<EE> \<ge> 0\<close>
+  unfolding kraus_family_norm_def
+  apply (rule cSUP_upper2[where x=\<open>{}\<close>])
+  using assms
+  by (simp_all add: bdd_above_def kraus_family_def)
+
 (* Strengthening of Nat.of_nat_0_le_iff: wider type. *)
 lemma of_nat_0_le_iff: \<open>of_nat x \<ge> (0::_::{ordered_ab_semigroup_add,zero_less_one})\<close>
   apply (induction x)
    apply auto
   by (metis add_mono semiring_norm(50) zero_less_one_class.zero_le_one)
 
-lemma sandwich_mono: \<open>sandwich A B \<le> sandwich A C\<close> if \<open>B \<le> C\<close>
-  by (metis cblinfun.real.diff_right diff_ge_0_iff_ge sandwich_pos that)
+lemma trace_class_sandwich: \<open>trace_class b \<Longrightarrow> trace_class (sandwich a b)\<close>
+  by (simp add: sandwich_apply trace_class_comp_right trace_class_comp_left)
+
+lemma trace_norm_butterfly: \<open>trace_norm (butterfly a a) = (norm a)^2\<close>
+  sorry
+
+lemma from_trace_class_sum:
+  shows \<open>from_trace_class (\<Sum>x\<in>M. f x) = (\<Sum>x\<in>M. from_trace_class (f x))\<close>
+  apply (induction M rule:infinite_finite_induct)
+  by (simp_all add: plus_trace_class.rep_eq)
+
+lemma not_not_singleton_zero: 
+  \<open>x = 0\<close> if \<open>\<not> class.not_singleton TYPE('a)\<close> for x :: \<open>'a::zero\<close>
+  using that unfolding class.not_singleton_def by auto
+
+lemma not_not_singleton_cblinfun_zero: 
+  \<open>x = 0\<close> if \<open>\<not> class.not_singleton TYPE('a)\<close> for x :: \<open>'a::complex_normed_vector \<Rightarrow>\<^sub>C\<^sub>L 'b::complex_normed_vector\<close>
+  apply (rule cblinfun_eqI)
+  apply (subst not_not_singleton_zero[OF that])
+  by simp
+
+(* lemma not_not_singleton_cblinfun_zero_simp:
+  \<open>x = 0\<close> if \<open>NO_MATCH 0 x\<close> \<open>\<not> class.not_singleton TYPE('a)\<close> for x :: \<open>'a::complex_normed_vector \<Rightarrow>\<^sub>C\<^sub>L 'b::complex_normed_vector\<close>
+  using that not_not_singleton_cblinfun_zero by simp *)
+
+lemma cblinfun_norm_approx_witness':
+  fixes A :: \<open>'a::complex_normed_vector \<Rightarrow>\<^sub>C\<^sub>L 'b::complex_normed_vector\<close>
+  assumes \<open>\<epsilon> > 0\<close>
+  shows \<open>\<exists>\<psi>. norm (A *\<^sub>V \<psi>) / norm \<psi> \<ge> norm A - \<epsilon>\<close>
+proof (cases \<open>class.not_singleton TYPE('a)\<close>)
+  case True
+  obtain \<psi> where \<open>norm (A *\<^sub>V \<psi>) \<ge> norm A - \<epsilon>\<close> and \<open>norm \<psi> = 1\<close>
+    apply atomize_elim
+    using complex_normed_vector_axioms True assms
+    by (rule cblinfun_norm_approx_witness[internalize_sort' 'a])
+  then have \<open>norm (A *\<^sub>V \<psi>) / norm \<psi> \<ge> norm A - \<epsilon>\<close>
+    by simp
+  then show ?thesis 
+    by auto
+next
+  case False
+  show ?thesis
+    apply (subst not_not_singleton_cblinfun_zero[OF False])
+     apply simp
+    apply (subst not_not_singleton_cblinfun_zero[OF False])
+    using \<open>\<epsilon> > 0\<close> by simp
+qed
+
+lemma any_norm_exists:
+  assumes \<open>n \<ge> 0\<close>
+  shows \<open>\<exists>\<psi>::'a::{real_normed_vector,not_singleton}. norm \<psi> = n\<close>
+proof -
+  obtain \<psi> :: 'a where \<open>\<psi> \<noteq> 0\<close>
+    using not_singleton_card
+    by force
+  then have \<open>norm (n *\<^sub>R sgn \<psi>) = n\<close>
+    using assms by (auto simp: sgn_div_norm abs_mult)
+  then show ?thesis
+    by blast
+qed
+
+lemma cblinfun_norm_approx_witness_cinner:
+  fixes A :: \<open>'a::{not_singleton,chilbert_space} \<Rightarrow>\<^sub>C\<^sub>L 'a\<close>
+  assumes \<open>A \<ge> 0\<close> and \<open>\<epsilon> > 0\<close>
+  shows \<open>\<exists>\<psi>. \<psi> \<bullet>\<^sub>C (A *\<^sub>V \<psi>) \<ge> norm A - \<epsilon> \<and> norm \<psi> = 1\<close>
+proof (cases \<open>A = 0\<close>)
+  case False
+  define B where \<open>B = sqrt_op A\<close>
+  define \<delta> where \<open>\<delta> = min (\<epsilon> / (2 * norm B)) (norm B)\<close>
+  then have \<open>\<delta> > 0\<close>
+    by (smt (verit, ccfv_threshold) B_def False Positive_Operators.sqrt_op_square assms(1) assms(2) linordered_field_class.divide_pos_pos norm_AAadj norm_eq_zero positive_hermitianI power_zero_numeral sqrt_op_pos zero_less_norm_iff)
+  have \<delta>: \<open>2 * (\<delta> * norm B) - \<delta> * \<delta> \<le> \<epsilon>\<close>
+  proof -
+    have \<open>\<delta> \<le> \<epsilon> / (2 * norm B)\<close>
+      by (simp add: \<delta>_def)
+  then show ?thesis
+    using assms(2) \<open>0 < \<delta>\<close>
+    by (smt (verit, best) Extra_Ordered_Fields.sign_simps(19) add_diff_cancel_left' diff_diff_eq2 less_eq_real_def linorder_not_less mult_le_cancel_left_pos nice_ordered_field_class.pos_le_divide_eq)
+  qed
+  from cblinfun_norm_approx_witness[OF \<open>\<delta> > 0\<close>]
+  obtain \<psi> where bound: \<open>norm B - \<delta> \<le> norm (B *\<^sub>V \<psi>)\<close> and \<open>norm \<psi> = 1\<close>
+    by auto
+  have \<open>complex_of_real (norm A - \<epsilon>) = (norm B)\<^sup>2 - \<epsilon>\<close>
+    by (metis B_def Positive_Operators.sqrt_op_square assms(1) norm_AAadj positive_hermitianI sqrt_op_pos)
+  also have \<open>\<dots> \<le> (norm B - \<delta>)^2\<close>
+    apply (rule complex_of_real_mono)
+    using \<delta> by (simp add: power2_eq_square left_diff_distrib right_diff_distrib)
+  also have \<open>\<dots> \<le> (norm (B *\<^sub>V \<psi>))^2\<close>
+    apply (rule complex_of_real_mono)
+    apply (rule power_mono)
+    apply (rule bound)
+    by (auto simp: \<delta>_def)
+  also have \<open>\<dots> = B \<psi> \<bullet>\<^sub>C B \<psi>\<close>
+    by (simp add: cdot_square_norm)
+  also have \<open>\<dots> = \<psi> \<bullet>\<^sub>C A \<psi>\<close>
+    by (metis B_def Positive_Operators.sqrt_op_square assms(1) cblinfun_apply_cblinfun_compose cinner_adj_right positive_hermitianI sqrt_op_pos)
+  finally show ?thesis
+    using \<open>norm \<psi> = 1\<close> by auto
+next
+  case True
+  with \<open>\<epsilon> > 0\<close> show ?thesis
+    by (auto intro!: any_norm_exists)
+qed
+
+lemma cblinfun_norm_approx_witness_cinner':
+  fixes A :: \<open>'a::chilbert_space \<Rightarrow>\<^sub>C\<^sub>L 'a\<close>
+  assumes \<open>A \<ge> 0\<close> and \<open>\<epsilon> > 0\<close>
+  shows \<open>\<exists>\<psi>. \<psi> \<bullet>\<^sub>C (A *\<^sub>V \<psi>) / (norm \<psi>)^2 \<ge> norm A - \<epsilon>\<close>
+proof (cases \<open>class.not_singleton TYPE('a)\<close>)
+  case True
+  obtain \<psi> where \<open>\<psi> \<bullet>\<^sub>C (A *\<^sub>V \<psi>) \<ge> norm A - \<epsilon>\<close> and \<open>norm \<psi> = 1\<close>
+    apply atomize_elim
+    using chilbert_space_axioms True assms
+    by (rule cblinfun_norm_approx_witness_cinner[internalize_sort' 'a])
+  then have \<open>\<psi> \<bullet>\<^sub>C (A *\<^sub>V \<psi>) / (norm \<psi>)^2 \<ge> norm A - \<epsilon>\<close>
+    by simp
+  then show ?thesis 
+    by auto
+next
+  case False
+  show ?thesis
+    apply (subst not_not_singleton_cblinfun_zero[OF False])
+     apply simp
+    apply (subst not_not_singleton_cblinfun_zero[OF False])
+    using \<open>\<epsilon> > 0\<close> by simp
+qed
+
+lemma bdd_above_mono2:
+  assumes \<open>bdd_above (g ` B)\<close>
+  assumes \<open>A \<subseteq> B\<close>
+  assumes \<open>\<And>x. x \<in> A \<Longrightarrow> f x \<le> g x\<close>
+  shows \<open>bdd_above (f ` A)\<close>
+  by (smt (verit, del_insts) Set.basic_monos(7) assms(1) assms(2) assms(3) basic_trans_rules(23) bdd_above.I2 bdd_above.unfold imageI)
+
+lemma has_sum_mono_neutral_complex:
+  fixes f :: "'a \<Rightarrow> complex"
+  assumes \<open>(f has_sum a) A\<close> and "(g has_sum b) B"
+  assumes \<open>\<And>x. x \<in> A\<inter>B \<Longrightarrow> f x \<le> g x\<close>
+  assumes \<open>\<And>x. x \<in> A-B \<Longrightarrow> f x \<le> 0\<close>
+  assumes \<open>\<And>x. x \<in> B-A \<Longrightarrow> g x \<ge> 0\<close>
+  shows "a \<le> b"
+proof -
+  have \<open>((\<lambda>x. Re (f x)) has_sum Re a) A\<close>
+    using assms(1) has_sum_Re has_sum_cong by blast
+  moreover have \<open>((\<lambda>x. Re (g x)) has_sum Re b) B\<close>
+    using assms(2) has_sum_Re has_sum_cong by blast
+  ultimately have Re: \<open>Re a \<le> Re b\<close>
+    apply (rule has_sum_mono_neutral)
+    using assms(3-5) by (simp_all add: less_eq_complex_def)
+  have \<open>((\<lambda>x. Im (f x)) has_sum Im a) A\<close>
+    using assms(1) has_sum_Im has_sum_cong by blast
+  then have \<open>((\<lambda>x. Im (f x)) has_sum Im a) (A \<inter> B)\<close>
+    apply (rule has_sum_cong_neutral[THEN iffD1, rotated -1])
+    using assms(3-5) by (auto simp add: less_eq_complex_def)
+  moreover have \<open>((\<lambda>x. Im (g x)) has_sum Im b) B\<close>
+    using assms(2) has_sum_Im has_sum_cong by blast
+  then have \<open>((\<lambda>x. Im (f x)) has_sum Im b) (A \<inter> B)\<close>
+    apply (rule has_sum_cong_neutral[THEN iffD1, rotated -1])
+    using assms(3-5) by (auto simp add: less_eq_complex_def)
+  ultimately have Im: \<open>Im a = Im b\<close>
+    by (rule has_sum_unique)
+  from Re Im show ?thesis
+    using less_eq_complexI by blast
+qed
+
+lemma has_sum_mono_neutral_wot:
+  fixes f :: "'a \<Rightarrow> ('b::chilbert_space \<Rightarrow>\<^sub>C\<^sub>L 'b)"
+  assumes \<open>has_sum_in cweak_operator_topology f A a\<close> and "has_sum_in cweak_operator_topology g B b"
+  assumes \<open>\<And>x. x \<in> A\<inter>B \<Longrightarrow> f x \<le> g x\<close>
+  assumes \<open>\<And>x. x \<in> A-B \<Longrightarrow> f x \<le> 0\<close>
+  assumes \<open>\<And>x. x \<in> B-A \<Longrightarrow> g x \<ge> 0\<close>
+  shows "a \<le> b"
+proof -
+  have \<psi>_eq: \<open>\<psi> \<bullet>\<^sub>C a \<psi> \<le> \<psi> \<bullet>\<^sub>C b \<psi>\<close> for \<psi>
+  proof -
+    from assms(1)
+    have sumA: \<open>((\<lambda>x. \<psi> \<bullet>\<^sub>C f x \<psi>) has_sum \<psi> \<bullet>\<^sub>C a \<psi>) A\<close>
+      by (simp add: has_sum_in_def has_sum_def limitin_cweak_operator_topology
+          cblinfun.sum_left cinner_sum_right)
+    from assms(2)
+    have sumB: \<open>((\<lambda>x. \<psi> \<bullet>\<^sub>C g x \<psi>) has_sum \<psi> \<bullet>\<^sub>C b \<psi>) B\<close>
+      by (simp add: has_sum_in_def has_sum_def limitin_cweak_operator_topology
+          cblinfun.sum_left cinner_sum_right)
+    from sumA sumB
+    show ?thesis
+      apply (rule has_sum_mono_neutral_complex)
+      using assms(3-5)
+      by (auto simp: less_eq_cblinfun_def)
+  qed
+  then show \<open>a \<le> b\<close>
+    by (simp add: less_eq_cblinfun_def)
+qed
+
+lemma sot_weaker_than_norm_limitin: \<open>limitin cstrong_operator_topology a A F\<close> if \<open>(a \<longlongrightarrow> A) F\<close>
+proof -
+  from that have \<open>((\<lambda>x. a x *\<^sub>V \<psi>) \<longlongrightarrow> A \<psi>) F\<close> for \<psi>
+    by (auto intro!: cblinfun.tendsto)
+  then show ?thesis
+    by (simp add: limitin_cstrong_operator_topology)
+qed
+
+(* lemma wot_weaker_than_traceclass_limitin: \<open>limitin cweak_operator_topology (\<lambda>x. from_trace_class (a x)) (from_trace_class A) F\<close> 
+  if \<open>(a \<longlongrightarrow> A) F\<close>
+proof -
+  from that have \<open>((\<lambda>x. a x *\<^sub>V \<psi>) \<longlongrightarrow> A \<psi>) F\<close> for \<psi>
+    by (auto intro!: cblinfun.tendsto) *)
+
+
+lemma has_sum_mono_neutral_traceclass:
+  fixes f :: "'a \<Rightarrow> ('b::chilbert_space, 'b) trace_class"
+  assumes \<open>(f has_sum a) A\<close> and "(g has_sum b) B"
+  assumes \<open>\<And>x. x \<in> A\<inter>B \<Longrightarrow> f x \<le> g x\<close>
+  assumes \<open>\<And>x. x \<in> A-B \<Longrightarrow> f x \<le> 0\<close>
+  assumes \<open>\<And>x. x \<in> B-A \<Longrightarrow> g x \<ge> 0\<close>
+  shows "a \<le> b"
+proof -
+  from assms(1)
+  have \<open>has_sum_in cweak_operator_topology (\<lambda>x. from_trace_class (f x)) A (from_trace_class a)\<close>
+    sorry
+  moreover
+  from assms(2)
+  have \<open>has_sum_in cweak_operator_topology (\<lambda>x. from_trace_class (g x)) B (from_trace_class b)\<close>
+    sorry
+  ultimately have \<open>from_trace_class a \<le> from_trace_class b\<close>
+    apply (rule has_sum_mono_neutral_wot)
+    using assms by (auto simp: less_eq_trace_class.rep_eq)
+  then show ?thesis
+    by (auto simp: less_eq_trace_class.rep_eq)
+qed
+
+lemma has_sum_mono_neutral_cblinfun:
+  fixes f :: "'a \<Rightarrow> ('b::chilbert_space \<Rightarrow>\<^sub>C\<^sub>L 'b)"
+  assumes \<open>(f has_sum a) A\<close> and "(g has_sum b) B"
+  assumes \<open>\<And>x. x \<in> A\<inter>B \<Longrightarrow> f x \<le> g x\<close>
+  assumes \<open>\<And>x. x \<in> A-B \<Longrightarrow> f x \<le> 0\<close>
+  assumes \<open>\<And>x. x \<in> B-A \<Longrightarrow> g x \<ge> 0\<close>
+  shows "a \<le> b"
+proof -
+  from assms(1)
+  have \<open>has_sum_in cweak_operator_topology f A a\<close> 
+    by (auto intro!: wot_weaker_than_sot_limitin sot_weaker_than_norm_limitin 
+        simp: has_sum_def has_sum_in_def)
+  moreover
+  from assms(2) have "has_sum_in cweak_operator_topology g B b"
+    by (auto intro!: wot_weaker_than_sot_limitin sot_weaker_than_norm_limitin 
+        simp: has_sum_def has_sum_in_def)
+  ultimately show ?thesis
+    apply (rule has_sum_mono_neutral_wot)
+    using assms by auto
+qed
+
+
+
+lemma has_sum_mono_cblinfun:
+  fixes f :: "'a \<Rightarrow> ('b::chilbert_space \<Rightarrow>\<^sub>C\<^sub>L 'b)"
+  assumes "(f has_sum x) A" and "(g has_sum y) A"
+  assumes \<open>\<And>x. x \<in> A \<Longrightarrow> f x \<le> g x\<close>
+  shows "x \<le> y"
+  using assms has_sum_mono_neutral_cblinfun by force
+
+lemma has_sum_mono_traceclass:
+  fixes f :: "'a \<Rightarrow> ('b::chilbert_space, 'b) trace_class"
+  assumes "(f has_sum x) A" and "(g has_sum y) A"
+  assumes \<open>\<And>x. x \<in> A \<Longrightarrow> f x \<le> g x\<close>
+  shows "x \<le> y"
+  using assms has_sum_mono_neutral_traceclass by force
+
+lemma infsum_mono_cblinfun:
+  fixes f :: "'a \<Rightarrow> ('b::chilbert_space \<Rightarrow>\<^sub>C\<^sub>L 'b)"
+  assumes "f summable_on A" and "g summable_on A"
+  assumes \<open>\<And>x. x \<in> A \<Longrightarrow> f x \<le> g x\<close>
+  shows "infsum f A \<le> infsum g A"
+  by (meson assms has_sum_infsum has_sum_mono_cblinfun)
+
+lemma infsum_mono_traceclass:
+  fixes f :: "'a \<Rightarrow> ('b::chilbert_space, 'b) trace_class"
+  assumes "f summable_on A" and "g summable_on A"
+  assumes \<open>\<And>x. x \<in> A \<Longrightarrow> f x \<le> g x\<close>
+  shows "infsum f A \<le> infsum g A"
+  by (meson assms has_sum_infsum has_sum_mono_traceclass)
+
+lemma infsum_mono_neutral_cblinfun:
+  fixes f :: "'a \<Rightarrow> ('b::chilbert_space \<Rightarrow>\<^sub>C\<^sub>L 'b)"
+  assumes "f summable_on A" and "g summable_on B"
+  assumes \<open>\<And>x. x \<in> A\<inter>B \<Longrightarrow> f x \<le> g x\<close>
+  assumes \<open>\<And>x. x \<in> A-B \<Longrightarrow> f x \<le> 0\<close>
+  assumes \<open>\<And>x. x \<in> B-A \<Longrightarrow> g x \<ge> 0\<close>
+  shows "infsum f A \<le> infsum g B"
+  by (smt (verit, del_insts) assms(1) assms(2) assms(3) assms(4) assms(5) has_sum_infsum has_sum_mono_neutral_cblinfun)
+
+lemma infsum_mono_neutral_traceclass:
+  fixes f :: "'a \<Rightarrow> ('b::chilbert_space, 'b) trace_class"
+  assumes "f summable_on A" and "g summable_on B"
+  assumes \<open>\<And>x. x \<in> A\<inter>B \<Longrightarrow> f x \<le> g x\<close>
+  assumes \<open>\<And>x. x \<in> A-B \<Longrightarrow> f x \<le> 0\<close>
+  assumes \<open>\<And>x. x \<in> B-A \<Longrightarrow> g x \<ge> 0\<close>
+  shows "infsum f A \<le> infsum g B"
+  using assms(1) assms(2) assms(3) assms(4) assms(5) has_sum_mono_neutral_traceclass summable_iff_has_sum_infsum by blast
+
+instance complex :: ordered_complex_vector
+  apply intro_classes
+  by (auto simp: less_eq_complex_def mult_left_mono mult_right_mono)
+
+instance cblinfun :: (chilbert_space, chilbert_space) ordered_complex_vector
+  by intro_classes
+
+instance trace_class :: (chilbert_space, chilbert_space) ordered_complex_vector
+  apply (intro_classes; transfer)
+  by (auto intro!: scaleC_left_mono scaleC_right_mono)
+
+lemma Abs_trace_class_geq0I: \<open>0 \<le> Abs_trace_class t\<close> if \<open>trace_class t\<close> and \<open>t \<ge> 0\<close>
+  sorry
+
+lemma kraus_family_map_abs_summable:
+  assumes \<open>kraus_family \<EE>\<close>
+  shows \<open>(\<lambda>E. of_nat (\<EE> E) *\<^sub>C Abs_trace_class (E o\<^sub>C\<^sub>L from_trace_class \<rho> o\<^sub>C\<^sub>L E*)) abs_summable_on UNIV\<close>
+(*
+proof -
+  wlog \<rho>_pos: \<open>\<rho> \<ge> 0\<close> generalizing \<rho>
+  proof -
+    have aux: \<open>trace_class (E o\<^sub>C\<^sub>L from_trace_class \<rho> o\<^sub>C\<^sub>L E* )\<close> 
+      for \<rho> :: \<open>('a, 'a) trace_class\<close> and E :: \<open>'a \<Rightarrow>\<^sub>C\<^sub>L 'b\<close>
+      by (simp add: trace_class_comp_left trace_class_comp_right)
+    obtain \<rho>1 \<rho>2 \<rho>3 \<rho>4 a1 a2 a3 a4 where \<rho>_decomp: \<open>\<rho> = a1 *\<^sub>C \<rho>1 + a2 *\<^sub>C \<rho>2 + a3 *\<^sub>C \<rho>3 + a4 *\<^sub>C \<rho>4\<close>
+      and pos: \<open>\<rho>1 \<ge> 0\<close> \<open>\<rho>2 \<ge> 0\<close> \<open>\<rho>3 \<ge> 0\<close> \<open>\<rho>4 \<ge> 0\<close>
+      by -
+    have \<open>norm (of_nat (\<EE> x) *\<^sub>C Abs_trace_class (x o\<^sub>C\<^sub>L from_trace_class \<rho> o\<^sub>C\<^sub>L x* )) 
+      \<le> norm (a1 *\<^sub>C of_nat (\<EE> x) *\<^sub>C Abs_trace_class (x o\<^sub>C\<^sub>L from_trace_class \<rho>1 o\<^sub>C\<^sub>L x* ))
+      + norm (a2 *\<^sub>C of_nat (\<EE> x) *\<^sub>C Abs_trace_class (x o\<^sub>C\<^sub>L from_trace_class \<rho>2 o\<^sub>C\<^sub>L x* ))
+      + norm (a3 *\<^sub>C of_nat (\<EE> x) *\<^sub>C Abs_trace_class (x o\<^sub>C\<^sub>L from_trace_class \<rho>3 o\<^sub>C\<^sub>L x* ))
+      + norm (a4 *\<^sub>C of_nat (\<EE> x) *\<^sub>C Abs_trace_class (x o\<^sub>C\<^sub>L from_trace_class \<rho>4 o\<^sub>C\<^sub>L x* ))\<close> 
+      (is \<open>_ \<le> ?S x\<close>) for x
+      apply (auto intro!: mult_left_mono
+          simp add: norm_trace_class.abs_eq eq_onp_def trace_class_plus trace_class_scaleC
+          aux trace_class_adj \<rho>_decomp plus_trace_class.rep_eq scaleC_trace_class.rep_eq
+          cblinfun_compose_add_right cblinfun_compose_add_left
+          scaleC_left_commute[of _ \<open>of_nat (\<EE> x)\<close>]
+          simp flip: ring_distribs
+          simp del: scaleC_scaleC)
+      by (smt (verit) local.aux trace_class_plus trace_class_scaleC trace_norm_scaleC trace_norm_triangle)
+    then have *: \<open>norm (of_nat (\<EE> x) *\<^sub>C Abs_trace_class (x o\<^sub>C\<^sub>L from_trace_class \<rho> o\<^sub>C\<^sub>L x* )) 
+      \<le> norm (?S x)\<close> for x
+      by force
+    show ?thesis
+      apply (rule abs_summable_on_comparison_test[OF _ *])
+      by (intro abs_summable_on_add abs_summable_norm abs_summable_on_scaleC_right hypothesis pos)
+  qed
+  have aux: \<open>trace_class (E o\<^sub>C\<^sub>L from_trace_class \<rho> o\<^sub>C\<^sub>L E* )\<close> 
+    for \<rho> :: \<open>('a, 'a) trace_class\<close> and E :: \<open>'a \<Rightarrow>\<^sub>C\<^sub>L 'b\<close>
+    by (simp add: trace_class_comp_left trace_class_comp_right)
+  define n\<rho> where \<open>n\<rho> = norm \<rho>\<close>
+  have *: \<open>norm (of_nat (\<EE> E) *\<^sub>C Abs_trace_class (E o\<^sub>C\<^sub>L from_trace_class \<rho> o\<^sub>C\<^sub>L E* ))
+      \<le> norm (norm \<rho> *\<^sub>C of_nat (\<EE> E) *\<^sub>C norm (E* o\<^sub>C\<^sub>L E))\<close> for E
+  proof -
+    have \<open>norm (Abs_trace_class (E o\<^sub>C\<^sub>L from_trace_class \<rho> o\<^sub>C\<^sub>L E* )) =
+          trace_norm (E o\<^sub>C\<^sub>L from_trace_class \<rho> o\<^sub>C\<^sub>L E* )\<close>
+      by (simp add: norm_trace_class.abs_eq eq_onp_def aux)
+    also have \<open>\<dots> = trace (E o\<^sub>C\<^sub>L from_trace_class \<rho> o\<^sub>C\<^sub>L E* )\<close>
+      by (metis \<rho>_pos abs_op_def from_trace_class_0 less_eq_trace_class.rep_eq sandwich_apply sandwich_pos sqrt_op_unique trace_abs_op)
+    also have \<open>\<dots> = trace (from_trace_class \<rho> o\<^sub>C\<^sub>L (E* o\<^sub>C\<^sub>L E))\<close>
+      by (simp add: Misc.lift_cblinfun_comp(2) circularity_of_trace trace_class_comp_left)
+    also have \<open>\<dots> \<le> trace_norm (from_trace_class \<rho>) * norm (E* o\<^sub>C\<^sub>L E)\<close>
+      by (metis Extra_Ordered_Fields.sign_simps(5) calculation circularity_of_trace cmod_trace_times complex_of_real_cmod complex_of_real_mono complex_of_real_nn_iff norm_ge_zero trace_class_from_trace_class)
+    also have \<open>\<dots> = norm \<rho> * norm (E* o\<^sub>C\<^sub>L E)\<close>
+      by (simp add: norm_trace_class.rep_eq)
+    finally show ?thesis
+  sledgehammer
+  by X (smt (verit, del_insts) Extra_Ordered_Fields.sign_simps(5) Extra_Ordered_Fields.sign_simps(6)
+ \<open>complex_of_real (trace_norm (E o\<^sub>C\<^sub>L from_trace_class \<rho> o\<^sub>C\<^sub>L E* )) = trace (E o\<^sub>C\<^sub>L from_trace_class \<rho> o\<^sub>C\<^sub>L E* )\<close> 
+\<open>norm (Abs_trace_class (E o\<^sub>C\<^sub>L from_trace_class \<rho> o\<^sub>C\<^sub>L E* )) = trace_norm (E o\<^sub>C\<^sub>L from_trace_class \<rho> o\<^sub>C\<^sub>L E* )\<close>
+ \<open>trace (E o\<^sub>C\<^sub>L from_trace_class \<rho> o\<^sub>C\<^sub>L E* ) = trace (from_trace_class \<rho> o\<^sub>C\<^sub>L (E* o\<^sub>C\<^sub>L E))\<close> 
+cmod_trace_times' mult_left_mono norm_AadjA norm_ge_zero 
+norm_mult norm_of_nat norm_of_real norm_trace_class.rep_eq of_real_power trace_class_from_trace_class)
+  try0
+  by -
+qed
+  from assms obtain B where B: \<open>norm (\<Sum>E\<in>S. \<EE> E *\<^sub>C (E* o\<^sub>C\<^sub>L E)) \<le> B\<close> if \<open>finite S\<close> for S
+    by (auto simp: kraus_family_def)
+
+  show ?thesis
+    apply (rule abs_summable_on_comparison_test[OF _ *])
+    apply (rule abs_summable_on_scaleC_right)
+(* TODO: Impossible goal here. E* o E only bounded in Loewner order, not in norm *)
+    apply (rule nonneg_bdd_above_summable_on, simp)
+    apply (rule bdd_aboveI[where M=B])
+    using B' apply safe
+  by -
+
+
+
+  show \<open>\<rho> \<ge> 0\<close>
+  sorry
+*)
+  sorry
+
+lemma kraus_family_map_summable:
+  assumes \<open>kraus_family \<EE>\<close>
+  shows \<open>(\<lambda>E. of_nat (\<EE> E) *\<^sub>C Abs_trace_class (sandwich E *\<^sub>V from_trace_class \<rho>)) summable_on UNIV\<close>
+  apply (rule abs_summable_summable)
+  unfolding sandwich_apply
+  using assms by (rule kraus_family_map_abs_summable)
+
+lemma kraus_family_map_bounded_tight:
+  assumes \<open>kraus_family \<EE>\<close>
+  shows \<open>kraus_family_norm \<EE> = (\<Squnion>\<rho>. norm (kraus_family_map \<EE> \<rho>) / norm \<rho>)\<close>
+proof (rule antisym)
+  from assms
+  have bounded: \<open>norm (kraus_family_map \<EE> \<rho>) / norm \<rho> \<le> kraus_family_norm \<EE>\<close> for \<rho>
+    apply (cases \<open>\<rho> = 0\<close>)
+    by (simp_all add: kraus_family_norm_geq0 kraus_family_map_bounded linordered_field_class.pos_divide_le_eq)
+
+  have aux1: \<open>0 \<le> (\<Sum>E\<in>M. complex_of_nat (\<EE> E) *\<^sub>C
+            Abs_trace_class (E o\<^sub>C\<^sub>L from_trace_class (Abs_trace_class (selfbutter \<psi>)) o\<^sub>C\<^sub>L E*))\<close> for \<psi> M
+    by (auto intro!: norm_cblinfun_mono sum_nonneg sum_mono
+        scaleC_nonneg_nonneg of_nat_0_le_iff Abs_trace_class_geq0I trace_class_sandwich sandwich_pos
+        simp: Abs_trace_class_inverse
+        simp flip: sandwich_apply)
+
+  show \<open>(\<Squnion>\<rho>. norm (kraus_family_map \<EE> \<rho>) / norm \<rho>) \<le> kraus_family_norm \<EE>\<close>
+    apply (rule cSUP_least)
+    using bounded by auto
+  show \<open>kraus_family_norm \<EE> \<le> (\<Squnion>\<rho>. norm (kraus_family_map \<EE> \<rho>) / norm \<rho>)\<close>
+    unfolding kraus_family_norm_def
+  proof (rule cSUP_least)
+    show \<open>Collect finite \<noteq> {}\<close>
+      by auto
+    fix M :: \<open>('a \<Rightarrow>\<^sub>C\<^sub>L 'b) set\<close>
+    assume \<open>M \<in> Collect finite\<close>
+    then have [simp]: \<open>finite M\<close> by simp
+    have \<open>norm (\<Sum>E\<in>M. complex_of_nat (\<EE> E) *\<^sub>C (E* o\<^sub>C\<^sub>L E)) - \<epsilon> \<le> (\<Squnion>\<rho>. norm (kraus_family_map \<EE> \<rho>) / norm \<rho>)\<close> 
+      (is \<open>?lhs \<le> ?rhs\<close>) if \<open>\<epsilon> > 0\<close> for \<epsilon>
+    proof (cases \<open>\<forall>\<psi>::'a. \<psi> = 0\<close>)
+      case True
+      then have *: \<open>(A::'a\<Rightarrow>\<^sub>C\<^sub>L'a) = 0\<close> for A
+        apply (rule_tac cblinfun_eqI)
+        by auto
+      show ?thesis
+        apply (rule cSUP_upper2[where x=0])
+        apply (rule bdd_aboveI[where M=\<open>kraus_family_norm \<EE>\<close>])
+        using bounded \<open>\<epsilon> > 0\<close> by (auto simp: *[of \<open>sum _ _\<close>])
+    next
+      case False
+      then have [simp]: \<open>class.not_singleton TYPE('a)\<close>
+        apply intro_classes by blast
+      obtain \<psi> where \<open>?lhs \<le> \<psi> \<bullet>\<^sub>C ((\<Sum>E\<in>M. complex_of_nat (\<EE> E) *\<^sub>C (E* o\<^sub>C\<^sub>L E)) *\<^sub>V \<psi>)\<close> and \<open>norm \<psi> = 1\<close>
+        apply atomize_elim
+        apply (rule cblinfun_norm_approx_witness_cinner[internalize_sort' 'a])
+        using \<open>\<epsilon> > 0\<close>
+        by (auto intro!: chilbert_space_axioms sum_nonneg scaleC_nonneg_nonneg of_nat_0_le_iff positive_cblinfun_squareI[OF refl])
+      then have \<open>?lhs \<le> \<psi> \<bullet>\<^sub>C ((\<Sum>E\<in>M. complex_of_nat (\<EE> E) *\<^sub>C (E* o\<^sub>C\<^sub>L E)) *\<^sub>V \<psi>)\<close> (* Just restating *)
+        by simp
+      also have \<open>\<dots> = trace ((\<Sum>E\<in>M. complex_of_nat (\<EE> E) *\<^sub>C (E* o\<^sub>C\<^sub>L E)) o\<^sub>C\<^sub>L selfbutter \<psi>)\<close>
+        by (simp flip: trace_butterfly_comp')
+      also have \<open>\<dots> = (\<Sum>E\<in>M. complex_of_nat (\<EE> E) * trace (E* o\<^sub>C\<^sub>L (E o\<^sub>C\<^sub>L selfbutter \<psi>)))\<close>
+        by (simp add: trace_class_scaleC trace_class_comp_right cblinfun_compose_sum_left
+            cblinfun_compose_assoc
+            flip: trace_scaleC trace_sum)
+      also have \<open>\<dots> = (\<Sum>E\<in>M. complex_of_nat (\<EE> E) * trace (sandwich E (selfbutter \<psi>)))\<close>
+        by (simp add: trace_class_comp_right sandwich_apply flip: circularity_of_trace)
+      also have \<open>\<dots> = trace (\<Sum>E\<in>M. complex_of_nat (\<EE> E) *\<^sub>C (sandwich E (selfbutter \<psi>)))\<close>
+        by (simp add: trace_class_scaleC trace_class_comp_right cblinfun_compose_assoc trace_class_sandwich
+            flip: trace_scaleC trace_sum)
+      also have \<open>\<dots> = trace_norm (\<Sum>E\<in>M. complex_of_nat (\<EE> E) *\<^sub>C (sandwich E (selfbutter \<psi>)))\<close>
+        by (simp_all add: sandwich_pos of_nat_0_le_iff scaleC_nonneg_nonneg sum_nonneg abs_op_id_on_pos
+            flip: trace_abs_op)
+      also have \<open>\<dots> \<le> norm (\<Sum>E\<in>M.
+             complex_of_nat (\<EE> E) *\<^sub>C Abs_trace_class (E o\<^sub>C\<^sub>L from_trace_class (Abs_trace_class (selfbutter \<psi>)) o\<^sub>C\<^sub>L E*))\<close>
+        by (simp add: norm_trace_class.rep_eq from_trace_class_sum scaleC_trace_class.rep_eq
+             Abs_trace_class_inverse trace_class_sandwich
+             flip: sandwich_apply)
+    
+(*       (* Experiment *)
+      have \<open>norm (\<Sum>E\<in>M.
+             complex_of_nat (\<EE> E) *\<^sub>C Abs_trace_class (E o\<^sub>C\<^sub>L from_trace_class (Abs_trace_class (selfbutter \<psi>)) o\<^sub>C\<^sub>L E* ))
+\<le> 
+norm (\<Sum>E\<in>UNIV.
+               complex_of_nat (\<EE> E) *\<^sub>C
+               Abs_trace_class (E o\<^sub>C\<^sub>L from_trace_class (Abs_trace_class (selfbutter \<psi>)) o\<^sub>C\<^sub>L E* ))
+\<close>
+        apply (rule norm_cblinfun_mono_trace_class)
+ *)
+
+      also have \<open>\<dots> \<le> norm (kraus_family_map \<EE> (Abs_trace_class (selfbutter \<psi>)))\<close>
+        apply (rule complex_of_real_mono)
+        unfolding kraus_family_map_def
+        using aux1 apply (rule norm_cblinfun_mono_trace_class)
+        apply (subst infsum_finite[symmetric], simp)
+        apply (rule infsum_mono_neutral_traceclass)
+            apply (auto intro!: aux1 scaleC_nonneg_nonneg of_nat_0_le_iff
+            Abs_trace_class_geq0I trace_class_sandwich sandwich_pos
+            kraus_family_map_summable \<open>kraus_family \<EE>\<close>
+            simp: summable_on_finite
+            simp flip: sandwich_apply Abs_trace_class_inverse)
+        using kraus_family_map_summable
+        by (simp add: Abs_trace_class_inverse)
+      also have \<open>\<dots> = norm (kraus_family_map \<EE> (Abs_trace_class (selfbutter \<psi>))) / norm (Abs_trace_class (selfbutter \<psi>))\<close>
+        by (simp add: norm_trace_class.abs_eq eq_onp_def trace_norm_butterfly \<open>norm \<psi> = 1\<close>)
+      also have \<open>\<dots> \<le> ?rhs\<close>
+        apply (rule complex_of_real_mono)
+        apply (rule cSup_upper)
+        apply simp
+        apply (rule bdd_aboveI[where M=\<open>kraus_family_norm \<EE>\<close>])
+        using bounded by auto
+      finally show ?thesis
+        using complex_of_real_mono_iff by blast
+    qed
+    then show \<open>norm (\<Sum>E\<in>M. complex_of_nat (\<EE> E) *\<^sub>C (E* o\<^sub>C\<^sub>L E)) \<le> (\<Squnion>\<rho>. norm (kraus_family_map \<EE> \<rho>) / norm \<rho>)\<close>
+      by (smt (verit, ccfv_SIG) nice_ordered_field_class.field_le_epsilon)
+  qed
+qed
+
+
+lemma
+  assumes \<open>kraus_family \<EE>\<close>
+  shows \<open>((\<lambda>F. norm (\<Sum>E\<in>F. complex_of_nat (\<EE> E) *\<^sub>C (E* o\<^sub>C\<^sub>L E))) \<longlongrightarrow> kraus_family_norm \<EE>) (finite_subsets_at_top UNIV)\<close>
+  sorry
+
+lemma kraus_family_norm_welldefined:
+  assumes \<open>kraus_equivalent \<EE> \<FF>\<close>
+  shows \<open>kraus_family_norm \<EE> = kraus_family_norm \<FF>\<close>
+  using assms unfolding kraus_equivalent_def
+  by (smt (z3) SUP_cong kraus_family_map_bounded_tight)
+
+lift_definition kraus_map_norm :: \<open>('a::chilbert_space, 'b::chilbert_space) kraus_map \<Rightarrow> real\<close> is
+  kraus_family_norm
+  by (rule kraus_family_norm_welldefined)
+
+lemma kraus_map_of_op_norm[simp]:
+  \<open>kraus_map_norm (kraus_map_of_op E) = (norm E)\<^sup>2\<close>
+  apply (transfer fixing: E)
+  by simp
 
 lemma less_eq_scaled_id_norm: 
   assumes \<open>norm A \<le> c\<close> and \<open>A = A*\<close>
@@ -280,93 +903,6 @@ lemma abs_summable_on_scaleC_right [intro]:
    apply simp
   by (auto intro!: summable_on_cmult_right assms simp: norm_scaleC)
 
-lemma kraus_family_map_abs_summable:
-  assumes \<open>kraus_family \<EE>\<close>
-  shows \<open>(\<lambda>E. of_nat (\<EE> E) *\<^sub>C Abs_trace_class (E o\<^sub>C\<^sub>L from_trace_class \<rho> o\<^sub>C\<^sub>L E*)) abs_summable_on UNIV\<close>
-(*
-proof -
-  wlog \<rho>_pos: \<open>\<rho> \<ge> 0\<close> generalizing \<rho>
-  proof -
-    have aux: \<open>trace_class (E o\<^sub>C\<^sub>L from_trace_class \<rho> o\<^sub>C\<^sub>L E* )\<close> 
-      for \<rho> :: \<open>('a, 'a) trace_class\<close> and E :: \<open>'a \<Rightarrow>\<^sub>C\<^sub>L 'b\<close>
-      by (simp add: trace_class_comp_left trace_class_comp_right)
-    obtain \<rho>1 \<rho>2 \<rho>3 \<rho>4 a1 a2 a3 a4 where \<rho>_decomp: \<open>\<rho> = a1 *\<^sub>C \<rho>1 + a2 *\<^sub>C \<rho>2 + a3 *\<^sub>C \<rho>3 + a4 *\<^sub>C \<rho>4\<close>
-      and pos: \<open>\<rho>1 \<ge> 0\<close> \<open>\<rho>2 \<ge> 0\<close> \<open>\<rho>3 \<ge> 0\<close> \<open>\<rho>4 \<ge> 0\<close>
-      by -
-    have \<open>norm (of_nat (\<EE> x) *\<^sub>C Abs_trace_class (x o\<^sub>C\<^sub>L from_trace_class \<rho> o\<^sub>C\<^sub>L x* )) 
-      \<le> norm (a1 *\<^sub>C of_nat (\<EE> x) *\<^sub>C Abs_trace_class (x o\<^sub>C\<^sub>L from_trace_class \<rho>1 o\<^sub>C\<^sub>L x* ))
-      + norm (a2 *\<^sub>C of_nat (\<EE> x) *\<^sub>C Abs_trace_class (x o\<^sub>C\<^sub>L from_trace_class \<rho>2 o\<^sub>C\<^sub>L x* ))
-      + norm (a3 *\<^sub>C of_nat (\<EE> x) *\<^sub>C Abs_trace_class (x o\<^sub>C\<^sub>L from_trace_class \<rho>3 o\<^sub>C\<^sub>L x* ))
-      + norm (a4 *\<^sub>C of_nat (\<EE> x) *\<^sub>C Abs_trace_class (x o\<^sub>C\<^sub>L from_trace_class \<rho>4 o\<^sub>C\<^sub>L x* ))\<close> 
-      (is \<open>_ \<le> ?S x\<close>) for x
-      apply (auto intro!: mult_left_mono
-          simp add: norm_trace_class.abs_eq eq_onp_def trace_class_plus trace_class_scaleC
-          aux trace_class_adj \<rho>_decomp plus_trace_class.rep_eq scaleC_trace_class.rep_eq
-          cblinfun_compose_add_right cblinfun_compose_add_left
-          scaleC_left_commute[of _ \<open>of_nat (\<EE> x)\<close>]
-          simp flip: ring_distribs
-          simp del: scaleC_scaleC)
-      by (smt (verit) local.aux trace_class_plus trace_class_scaleC trace_norm_scaleC trace_norm_triangle)
-    then have *: \<open>norm (of_nat (\<EE> x) *\<^sub>C Abs_trace_class (x o\<^sub>C\<^sub>L from_trace_class \<rho> o\<^sub>C\<^sub>L x* )) 
-      \<le> norm (?S x)\<close> for x
-      by force
-    show ?thesis
-      apply (rule abs_summable_on_comparison_test[OF _ *])
-      by (intro abs_summable_on_add abs_summable_norm abs_summable_on_scaleC_right hypothesis pos)
-  qed
-  have aux: \<open>trace_class (E o\<^sub>C\<^sub>L from_trace_class \<rho> o\<^sub>C\<^sub>L E* )\<close> 
-    for \<rho> :: \<open>('a, 'a) trace_class\<close> and E :: \<open>'a \<Rightarrow>\<^sub>C\<^sub>L 'b\<close>
-    by (simp add: trace_class_comp_left trace_class_comp_right)
-  define n\<rho> where \<open>n\<rho> = norm \<rho>\<close>
-  have *: \<open>norm (of_nat (\<EE> E) *\<^sub>C Abs_trace_class (E o\<^sub>C\<^sub>L from_trace_class \<rho> o\<^sub>C\<^sub>L E* ))
-      \<le> norm (norm \<rho> *\<^sub>C of_nat (\<EE> E) *\<^sub>C norm (E* o\<^sub>C\<^sub>L E))\<close> for E
-  proof -
-    have \<open>norm (Abs_trace_class (E o\<^sub>C\<^sub>L from_trace_class \<rho> o\<^sub>C\<^sub>L E* )) =
-          trace_norm (E o\<^sub>C\<^sub>L from_trace_class \<rho> o\<^sub>C\<^sub>L E* )\<close>
-      by (simp add: norm_trace_class.abs_eq eq_onp_def aux)
-    also have \<open>\<dots> = trace (E o\<^sub>C\<^sub>L from_trace_class \<rho> o\<^sub>C\<^sub>L E* )\<close>
-      by (metis \<rho>_pos abs_op_def from_trace_class_0 less_eq_trace_class.rep_eq sandwich_apply sandwich_pos sqrt_op_unique trace_abs_op)
-    also have \<open>\<dots> = trace (from_trace_class \<rho> o\<^sub>C\<^sub>L (E* o\<^sub>C\<^sub>L E))\<close>
-      by (simp add: Misc.lift_cblinfun_comp(2) circularity_of_trace trace_class_comp_left)
-    also have \<open>\<dots> \<le> trace_norm (from_trace_class \<rho>) * norm (E* o\<^sub>C\<^sub>L E)\<close>
-      by (metis Extra_Ordered_Fields.sign_simps(5) calculation circularity_of_trace cmod_trace_times complex_of_real_cmod complex_of_real_mono complex_of_real_nn_iff norm_ge_zero trace_class_from_trace_class)
-    also have \<open>\<dots> = norm \<rho> * norm (E* o\<^sub>C\<^sub>L E)\<close>
-      by (simp add: norm_trace_class.rep_eq)
-    finally show ?thesis
-  sledgehammer
-  by X (smt (verit, del_insts) Extra_Ordered_Fields.sign_simps(5) Extra_Ordered_Fields.sign_simps(6)
- \<open>complex_of_real (trace_norm (E o\<^sub>C\<^sub>L from_trace_class \<rho> o\<^sub>C\<^sub>L E* )) = trace (E o\<^sub>C\<^sub>L from_trace_class \<rho> o\<^sub>C\<^sub>L E* )\<close> 
-\<open>norm (Abs_trace_class (E o\<^sub>C\<^sub>L from_trace_class \<rho> o\<^sub>C\<^sub>L E* )) = trace_norm (E o\<^sub>C\<^sub>L from_trace_class \<rho> o\<^sub>C\<^sub>L E* )\<close>
- \<open>trace (E o\<^sub>C\<^sub>L from_trace_class \<rho> o\<^sub>C\<^sub>L E* ) = trace (from_trace_class \<rho> o\<^sub>C\<^sub>L (E* o\<^sub>C\<^sub>L E))\<close> 
-cmod_trace_times' mult_left_mono norm_AadjA norm_ge_zero 
-norm_mult norm_of_nat norm_of_real norm_trace_class.rep_eq of_real_power trace_class_from_trace_class)
-  try0
-  by -
-qed
-  from assms obtain B where B: \<open>norm (\<Sum>E\<in>S. \<EE> E *\<^sub>C (E* o\<^sub>C\<^sub>L E)) \<le> B\<close> if \<open>finite S\<close> for S
-    by (auto simp: kraus_family_def)
-
-  show ?thesis
-    apply (rule abs_summable_on_comparison_test[OF _ *])
-    apply (rule abs_summable_on_scaleC_right)
-(* TODO: Impossible goal here. E* o E only bounded in Loewner order, not in norm *)
-    apply (rule nonneg_bdd_above_summable_on, simp)
-    apply (rule bdd_aboveI[where M=B])
-    using B' apply safe
-  by -
-
-
-
-  show \<open>\<rho> \<ge> 0\<close>
-  sorry
-*)
-  sorry
-
-lemma kraus_family_map_summable:
-  assumes \<open>kraus_family \<EE>\<close>
-  shows \<open>(\<lambda>E. of_nat (\<EE> E) *\<^sub>C Abs_trace_class (E o\<^sub>C\<^sub>L from_trace_class \<rho> o\<^sub>C\<^sub>L E*)) summable_on UNIV\<close>
-  apply (rule abs_summable_summable)
-  using assms by (rule kraus_family_map_abs_summable)
 
 lemma kraus_family_comp_apply:
   assumes \<open>kraus_family \<EE>\<close> and \<open>kraus_family \<FF>\<close>
@@ -379,123 +915,6 @@ lift_definition kraus_map_comp :: \<open>('a::chilbert_space,'b::chilbert_space)
   by (auto intro!: kraus_family_kraus_family_comp
       simp add: kraus_equivalent_def kraus_family_comp_apply)
 
-
-datatype raw_program =
-  Seq \<open>raw_program\<close> \<open>raw_program\<close>
-  | Skip
-  | Sample \<open>cl distr expression\<close>
-  | IfThenElse \<open>bool expression\<close> \<open>raw_program\<close> \<open>raw_program\<close>
-  | While \<open>bool expression\<close> \<open>raw_program\<close>
-  | QuantumOp \<open>(qu ell2, qu ell2) kraus_map expression\<close>
-  | Measurement \<open>(cl, qu) measurement expression\<close>
-  | InstantiateOracles \<open>raw_program\<close> \<open>raw_program list\<close>
-(* TODO: Localvars *)
-  
-axiomatization valid_program :: \<open>raw_program \<Rightarrow> bool\<close>
-axiomatization valid_oracle_program :: \<open>raw_program \<Rightarrow> bool\<close>
-
-typedef program = \<open>Collect valid_program\<close>
-  sorry
-setup_lifting type_definition_program
-
-typedef oracle_program = \<open>Collect valid_oracle_program\<close>
-  sorry
-setup_lifting type_definition_oracle_program
-
-lift_definition oracle_program_from_program :: \<open>program \<Rightarrow> oracle_program\<close> is id
-  sorry
-
-lift_definition block :: \<open>program list \<Rightarrow> program\<close> is
-  \<open>\<lambda>ps. fold Seq ps Skip\<close>
-  sorry
-
-lift_definition sample :: \<open>'a cvariable \<Rightarrow> 'a distr expression \<Rightarrow> program\<close> is
-  \<open>\<lambda>X e. Sample (\<lambda>m::cl. map_distr (\<lambda>x. setter X x m) (e m))\<close>
-  sorry
-
-definition assign :: \<open>'a cvariable \<Rightarrow> 'a expression \<Rightarrow> program\<close> where
-  \<open>assign x e = sample x (point_distr o e)\<close>
-
-lift_definition qapply :: \<open>'a qvariable \<Rightarrow> ('a,'a) l2bounded expression \<Rightarrow> program\<close> is
-  \<open>\<lambda>Q e. QuantumOp (\<lambda>m. kraus_map_of_op (apply_qregister Q (e m)))\<close>
-  sorry
-
-consts
-  ifthenelse :: "bool expression \<Rightarrow> program list \<Rightarrow> program list \<Rightarrow> program"
-  while :: "bool expression \<Rightarrow> program list \<Rightarrow> program"
-  qinit :: "'a qvariable \<Rightarrow> 'a ell2 expression \<Rightarrow> program"
-  measurement :: "'a cvariable \<Rightarrow> 'b qvariable \<Rightarrow> ('a,'b) measurement expression \<Rightarrow> program"
-  instantiateOracles :: "oracle_program \<Rightarrow> program list \<Rightarrow> program"
-  localvars :: "'a cvariable \<Rightarrow> 'b qvariable \<Rightarrow> program list \<Rightarrow> program"
-
-consts fvq_program :: "program \<Rightarrow> QVARIABLE"
-consts fvc_program :: "program \<Rightarrow> CVARIABLE"
-consts fvcw_program :: "program \<Rightarrow> CVARIABLE"
-consts fvq_oracle_program :: "oracle_program \<Rightarrow> QVARIABLE"
-consts fvc_oracle_program :: "oracle_program \<Rightarrow> CVARIABLE"
-consts fvcw_oracle_program :: "oracle_program \<Rightarrow> CVARIABLE"
-
-(* consts fvq_program :: "program \<Rightarrow> string set" *)
-lemma fvq_program_sequence: "fvq_program (block b) = fold (\<lambda>p v. QREGISTER_pair (fvq_program p) v) b QREGISTER_unit"
-  sorry
-lemma fvq_program_assign: "fvq_program (assign x e) = QREGISTER_unit"
-  sorry
-lemma fvq_program_sample: "fvq_program (sample xs e2) = QREGISTER_unit"
-  sorry
-lemma fvq_program_ifthenelse: "fvq_program (ifthenelse c p1 p2) =
-  QREGISTER_pair (fvq_program (block p1)) (fvq_program (block p2))"
-  sorry
-lemma fvq_program_while: "fvq_program (while c b) = (fvq_program (block b))"
-  sorry
-lemma fvq_program_qinit: "fvq_program (qinit Q e3) = QREGISTER_of Q"
-  sorry
-lemma fvq_program_qapply: "fvq_program (qapply Q e4) = QREGISTER_of Q"
-  sorry
-lemma fvq_program_measurement: "fvq_program (measurement x R e5) = QREGISTER_of R"
-  sorry
-
-lemma fvc_program_sequence: "fvc_program (block b) = fold (\<lambda>p v. CREGISTER_pair (fvc_program p) v) b CREGISTER_unit"
-  sorry
-lemma fvc_program_assign: "fvc_program (assign x e) = CREGISTER_pair (CREGISTER_of x) (fv_expression e)"
-  sorry
-lemma fvc_program_sample: "fvc_program (sample x e) = CREGISTER_pair (CREGISTER_of x) (fv_expression e)"
-  sorry
-lemma fvc_program_ifthenelse: "fvc_program (ifthenelse c p1 p2) =
-  CREGISTER_pair (fv_expression c) (CREGISTER_pair (fvc_program (block p1)) (fvc_program (block p2)))"
-  sorry
-lemma fvc_program_while: "fvc_program (while c b) = 
-  CREGISTER_pair (fv_expression c) (fvc_program (block b))"
-  sorry
-lemma fvc_program_qinit: "fvc_program (qinit Q e3) = fv_expression e3"
-  sorry
-lemma fvc_program_qapply: "fvc_program (qapply Q e4) = fv_expression e4"
-  sorry
-lemma fvc_program_measurement: "fvc_program (measurement x R e) = CREGISTER_pair (CREGISTER_of x) (fv_expression e)"
-  sorry
-
-lemma fvcw_program_sequence: "fvcw_program (block b) = fold (\<lambda>p v. CREGISTER_pair (fvcw_program p) v) b CREGISTER_unit"
-  sorry
-lemma fvcw_program_assign: "fvcw_program (assign x e) = CREGISTER_of x"
-  sorry
-lemma fvcw_program_sample: "fvcw_program (sample x e2) = CREGISTER_of x"
-  sorry
-lemma fvcw_program_ifthenelse: "fvcw_program (ifthenelse c p1 p2) =
-  CREGISTER_pair (fvc_program (block p1)) (fvc_program (block p2))"
-  sorry
-lemma fvcw_program_while: "fvcw_program (while c b) = fvcw_program (block b)"
-  sorry
-lemma fvcw_program_qinit: "fvcw_program (qinit Q e3) = CREGISTER_unit"
-  sorry
-lemma fvcw_program_qapply: "fvcw_program (qapply Q e4) = CREGISTER_unit"
-  sorry
-lemma fvcw_program_measurement: "fvcw_program (measurement x R e5) = CREGISTER_of x"
-  sorry
-
-lemma localvars_empty: "localvars empty_cregister empty_qregister P = block P"
-  sorry
-
-lemma singleton_block: "block [P] = P"
-  sorry
 
 (* TODO replace original *) thm norm_leq_trace_norm
 lemma norm_leq_trace_norm: \<open>norm t \<le> trace_norm t\<close> if \<open>trace_class t\<close> 
@@ -842,10 +1261,203 @@ proof intro_classes
 qed
 end
 
+definition \<open>kraus_map_id = kraus_map_of_op id_cblinfun\<close>
+
+instantiation kraus_map :: (chilbert_space, chilbert_space) comm_monoid_add begin
+lift_definition zero_kraus_map :: \<open>('a,'b) kraus_map\<close> is \<open>\<lambda>_. 0::nat\<close>
+  by (simp add: kraus_equivalent_def)
+lift_definition plus_kraus_map :: \<open>('a,'b) kraus_map \<Rightarrow> ('a,'b) kraus_map \<Rightarrow> ('a,'b) kraus_map\<close> is
+  \<open>\<lambda>a b x. a x + b x\<close>
+  apply (simp add: kraus_equivalent_def)
+  sorry
+instance
+  sorry
+end
+
+
+datatype raw_program =
+  Seq \<open>raw_program\<close> \<open>raw_program\<close>
+  | Skip
+  | Sample \<open>cl distr expression\<close>
+  | IfThenElse \<open>bool expression\<close> \<open>raw_program\<close> \<open>raw_program\<close>
+  | While \<open>bool expression\<close> \<open>raw_program\<close>
+  | QuantumOp \<open>(qu ell2, qu ell2) kraus_map expression\<close>
+  | Measurement \<open>(cl, qu) measurement expression\<close>
+  | InstantiateOracles \<open>raw_program\<close> \<open>raw_program list\<close>
+  | LocalQ \<open>qu QREGISTER\<close> \<open>(qu ell2, qu ell2) trace_class\<close> \<open>raw_program\<close>
+  | LocalC \<open>cl CREGISTER\<close> \<open>cl \<Rightarrow> cl\<close> \<open>raw_program\<close>
+  | OracleCall nat
+
+fun oracle_number :: \<open>raw_program \<Rightarrow> nat\<close> where
+  \<open>oracle_number (Seq c d) = max (oracle_number c) (oracle_number d)\<close>
+| \<open>oracle_number Skip = 0\<close>
+| \<open>oracle_number (Sample _) = 0\<close>
+| \<open>oracle_number (QuantumOp _) = 0\<close>
+| \<open>oracle_number (Measurement _) = 0\<close>
+| \<open>oracle_number (IfThenElse e c d) = max (oracle_number c) (oracle_number d)\<close>
+| \<open>oracle_number (While e c) = oracle_number c\<close>
+| \<open>oracle_number (InstantiateOracles _ _) = 0\<close>
+| \<open>oracle_number (LocalQ _ _ c) = oracle_number c\<close>
+| \<open>oracle_number (LocalC _ _ c) = oracle_number c\<close>
+| \<open>oracle_number (OracleCall i) = Suc i\<close>
+
+
+inductive valid_oracle_program :: \<open>raw_program \<Rightarrow> bool\<close> and valid_program :: \<open>raw_program \<Rightarrow> bool\<close> where
+  \<open>valid_oracle_program c \<Longrightarrow> valid_oracle_program d \<Longrightarrow> valid_oracle_program (Seq c d)\<close>
+| \<open>valid_oracle_program Skip\<close>
+| \<open>(\<And>m. weight (e m) \<le> 1) \<Longrightarrow> valid_oracle_program (Sample e)\<close>
+| \<open>valid_oracle_program c \<Longrightarrow> valid_oracle_program d \<Longrightarrow> valid_oracle_program (IfThenElse e c d)\<close>
+| \<open>valid_oracle_program c \<Longrightarrow> valid_oracle_program (While e c)\<close>
+| \<open>(\<And>m. kraus_map_norm (e m) \<le> 1) \<Longrightarrow> valid_oracle_program (QuantumOp e)\<close>
+| \<open>valid_oracle_program (Measurement e)\<close>
+| \<open>(\<And>d. d \<in> set ds \<Longrightarrow> valid_program d) \<Longrightarrow> valid_oracle_program c \<Longrightarrow> 
+  oracle_number c \<le> length ds \<Longrightarrow> valid_oracle_program (InstantiateOracles c ds)\<close>
+| \<open>valid_oracle_program c \<Longrightarrow> ACTUAL_QREGISTER q \<Longrightarrow> norm \<rho> = 1 \<Longrightarrow> from_trace_class \<rho> \<in> Rep_QREGISTER q \<Longrightarrow> valid_oracle_program (LocalQ q \<rho> c)\<close>
+| \<open>valid_oracle_program c \<Longrightarrow> Some o f \<in> Rep_CREGISTER x \<Longrightarrow> 
+    (\<And>g. Some o g \<in> Rep_CREGISTER x \<Longrightarrow> f o g = f) \<Longrightarrow> valid_oracle_program (LocalC x f c)\<close>
+| \<open>valid_oracle_program c \<Longrightarrow> oracle_number c = 0 \<Longrightarrow> valid_program c\<close>
+
+
+typedef program = \<open>Collect valid_program\<close>
+  apply (rule exI[of _ Skip])
+  by (simp add: valid_oracle_program_valid_program.intros)
+setup_lifting type_definition_program
+
+typedef oracle_program = \<open>Collect valid_oracle_program\<close>
+  apply (rule exI[of _ Skip])
+  by (simp add: valid_oracle_program_valid_program.intros)
+setup_lifting type_definition_oracle_program
+
+lift_definition oracle_program_from_program :: \<open>program \<Rightarrow> oracle_program\<close> is id
+  by (simp add: valid_program.simps)
+
+lift_definition block :: \<open>program list \<Rightarrow> program\<close> is
+  \<open>\<lambda>ps. fold Seq ps Skip\<close>
+proof -
+  fix ps
+  assume \<open>list_all (\<lambda>x. x \<in> Collect valid_program) ps\<close>
+  then have \<open>list_all valid_program ps\<close>
+    by simp
+  then have \<open>valid_oracle_program (fold Seq ps Skip)\<close> and \<open>oracle_number (fold Seq ps Skip) = 0\<close>
+  proof (induction ps rule:rev_induct)
+    case Nil
+    show \<open>valid_oracle_program (fold Seq [] Skip)\<close>
+      by (auto intro!: valid_oracle_program_valid_program.intros)
+    show \<open>oracle_number (fold Seq [] Skip) = 0\<close>
+      by simp
+  next
+    case (snoc p ps)
+    then show \<open>valid_oracle_program (fold Seq (ps @ [p]) Skip)\<close>
+      if \<open>list_all valid_program (ps @ [p])\<close>
+      using that apply (auto intro!: valid_oracle_program_valid_program.intros)
+      using valid_program.simps by blast
+    show \<open>oracle_number (fold Seq (ps @ [p]) Skip) = 0\<close>
+      if \<open>list_all valid_program (ps @ [p])\<close>
+      using that snoc apply simp
+      using valid_program.simps by blast
+  qed
+  then show \<open>fold Seq ps Skip \<in> Collect valid_program\<close>
+    by (simp add: valid_program.simps)
+qed
+
+lift_definition sample :: \<open>'a cvariable \<Rightarrow> 'a distr expression \<Rightarrow> program\<close> is
+  \<open>\<lambda>X e. Sample (\<lambda>m::cl. map_distr (\<lambda>x. setter X x m) (e m))\<close>
+  by (simp add: valid_oracle_program_valid_program.intros(3) valid_program.simps)
+
+definition assign :: \<open>'a cvariable \<Rightarrow> 'a expression \<Rightarrow> program\<close> where
+  \<open>assign x e = sample x (point_distr o e)\<close>
+
+lift_definition qapply :: \<open>'a qvariable \<Rightarrow> ('a,'a) l2bounded expression \<Rightarrow> program\<close> is
+  \<open>\<lambda>Q e. if qregister Q then
+      QuantumOp (\<lambda>m. kraus_map_of_op (apply_qregister Q (if norm (e m) \<le> 1 then e m else 0))) else Skip\<close>
+  apply (auto intro!: valid_oracle_program_valid_program.intros)
+  by (simp add: power_le_one)
+
+consts
+  ifthenelse :: "bool expression \<Rightarrow> program list \<Rightarrow> program list \<Rightarrow> program"
+  while :: "bool expression \<Rightarrow> program list \<Rightarrow> program"
+  qinit :: "'a qvariable \<Rightarrow> 'a ell2 expression \<Rightarrow> program"
+  measurement :: "'a cvariable \<Rightarrow> 'b qvariable \<Rightarrow> ('a,'b) measurement expression \<Rightarrow> program"
+  instantiateOracles :: "oracle_program \<Rightarrow> program list \<Rightarrow> program"
+  localvars :: "'a cvariable \<Rightarrow> 'b qvariable \<Rightarrow> program list \<Rightarrow> program"
+
+consts fvq_program :: "program \<Rightarrow> QVARIABLE"
+consts fvc_program :: "program \<Rightarrow> CVARIABLE"
+consts fvcw_program :: "program \<Rightarrow> CVARIABLE"
+consts fvq_oracle_program :: "oracle_program \<Rightarrow> QVARIABLE"
+consts fvc_oracle_program :: "oracle_program \<Rightarrow> CVARIABLE"
+consts fvcw_oracle_program :: "oracle_program \<Rightarrow> CVARIABLE"
+
+(* consts fvq_program :: "program \<Rightarrow> string set" *)
+lemma fvq_program_sequence: "fvq_program (block b) = fold (\<lambda>p v. QREGISTER_pair (fvq_program p) v) b QREGISTER_unit"
+  sorry
+lemma fvq_program_assign: "fvq_program (assign x e) = QREGISTER_unit"
+  sorry
+lemma fvq_program_sample: "fvq_program (sample xs e2) = QREGISTER_unit"
+  sorry
+lemma fvq_program_ifthenelse: "fvq_program (ifthenelse c p1 p2) =
+  QREGISTER_pair (fvq_program (block p1)) (fvq_program (block p2))"
+  sorry
+lemma fvq_program_while: "fvq_program (while c b) = (fvq_program (block b))"
+  sorry
+lemma fvq_program_qinit: "fvq_program (qinit Q e3) = QREGISTER_of Q"
+  sorry
+lemma fvq_program_qapply: "fvq_program (qapply Q e4) = QREGISTER_of Q"
+  sorry
+lemma fvq_program_measurement: "fvq_program (measurement x R e5) = QREGISTER_of R"
+  sorry
+
+lemma fvc_program_sequence: "fvc_program (block b) = fold (\<lambda>p v. CREGISTER_pair (fvc_program p) v) b CREGISTER_unit"
+  sorry
+lemma fvc_program_assign: "fvc_program (assign x e) = CREGISTER_pair (CREGISTER_of x) (fv_expression e)"
+  sorry
+lemma fvc_program_sample: "fvc_program (sample x e) = CREGISTER_pair (CREGISTER_of x) (fv_expression e)"
+  sorry
+lemma fvc_program_ifthenelse: "fvc_program (ifthenelse c p1 p2) =
+  CREGISTER_pair (fv_expression c) (CREGISTER_pair (fvc_program (block p1)) (fvc_program (block p2)))"
+  sorry
+lemma fvc_program_while: "fvc_program (while c b) = 
+  CREGISTER_pair (fv_expression c) (fvc_program (block b))"
+  sorry
+lemma fvc_program_qinit: "fvc_program (qinit Q e3) = fv_expression e3"
+  sorry
+lemma fvc_program_qapply: "fvc_program (qapply Q e4) = fv_expression e4"
+  sorry
+lemma fvc_program_measurement: "fvc_program (measurement x R e) = CREGISTER_pair (CREGISTER_of x) (fv_expression e)"
+  sorry
+
+lemma fvcw_program_sequence: "fvcw_program (block b) = fold (\<lambda>p v. CREGISTER_pair (fvcw_program p) v) b CREGISTER_unit"
+  sorry
+lemma fvcw_program_assign: "fvcw_program (assign x e) = CREGISTER_of x"
+  sorry
+lemma fvcw_program_sample: "fvcw_program (sample x e2) = CREGISTER_of x"
+  sorry
+lemma fvcw_program_ifthenelse: "fvcw_program (ifthenelse c p1 p2) =
+  CREGISTER_pair (fvc_program (block p1)) (fvc_program (block p2))"
+  sorry
+lemma fvcw_program_while: "fvcw_program (while c b) = fvcw_program (block b)"
+  sorry
+lemma fvcw_program_qinit: "fvcw_program (qinit Q e3) = CREGISTER_unit"
+  sorry
+lemma fvcw_program_qapply: "fvcw_program (qapply Q e4) = CREGISTER_unit"
+  sorry
+lemma fvcw_program_measurement: "fvcw_program (measurement x R e5) = CREGISTER_of x"
+  sorry
+
+lemma localvars_empty: "localvars empty_cregister empty_qregister P = block P"
+  sorry
+
+lemma singleton_block: "block [P] = P"
+  sorry
+
 type_synonym program_state = \<open>(cl,qu) cq_operator\<close>
 
-axiomatization
-  denotation :: "program \<Rightarrow> program_state \<Rightarrow> program_state"
+fun denotation_raw :: "raw_program \<Rightarrow> program_state \<Rightarrow> program_state" where
+  denotation_raw_Skip: \<open>denotation_raw Skip \<rho> = \<rho>\<close>
+| denotation_raw_Seq: \<open>denotation_raw (Seq c d) \<rho> = denotation_raw d (denotation_raw c \<rho>)\<close>
+(* TODO missing cases *)
+
+lift_definition denotation :: "program \<Rightarrow> program_state \<Rightarrow> program_state" is denotation_raw.
 
 lift_definition program_state_distrib :: "program_state \<Rightarrow> cl distr" is
   \<open>\<lambda>\<rho> m. if \<rho> \<ge> 0 \<and> norm \<rho> \<le> 1 then norm (cq_operator_at \<rho> m) else 0\<close>
@@ -867,8 +1479,12 @@ proof -
   qed
 qed
 
-lemma denotation_block: "denotation (block ps) = fold denotation ps"
-  sorry
+lemma denotation_block: "denotation (block ps) = foldr denotation ps"
+  apply transfer
+  subgoal for ps
+    apply (induction ps rule:rev_induct)
+    by (auto intro!: ext)
+  done
 
 definition probability :: "bool expression \<Rightarrow> program \<Rightarrow> program_state \<Rightarrow> real" where
   "probability e p \<rho> = Prob (program_state_distrib (denotation p \<rho>)) (Collect e)"
